ironfleet/src/Dafny/Distributed/Services/SHT/SHTDistributedSystem.i.dfy
@@ -1,8 +1,62 @@
 include "../../Impl/LiveSHT/Host.i.dfy"
-include "../../Common/Framework/DistributedSystem.s.dfy"
+// include "../../Common/Framework/DistributedSystem.s.dfy"
 
-module SHT_DistributedSystem_i refines DistributedSystem_s {
+module SHT_DistributedSystem_i {
 
-    import H_s = Host_i`All
+    // import H_s = Host_i`All
+import H_s  = Host_i`All
+import opened Collections__Maps2_s
+import opened Native__Io_s
+import opened Environment_s
+import opened Native__NativeTypes_s
 
+/////////////////////////////////////////
+// PHYSICAL ENVIRONMENT
+/////////////////////////////////////////
+
+predicate ValidPhysicalEnvironmentStep(step:LEnvStep<EndPoint, seq<byte>>)
+{
+  step.LEnvStepHostIos? ==> forall io{:trigger io in step.ios}{:trigger ValidPhysicalIo(io)} :: io in step.ios ==> ValidPhysicalIo(io)
+}
+
+/////////////////////////////////////////
+// DS_State
+/////////////////////////////////////////
+
+datatype DS_State = DS_State(
+  config:H_s.ConcreteConfiguration,
+  environment:LEnvironment<EndPoint,seq<byte>>,
+  servers:map<EndPoint,H_s.HostState>
+  )
+
+predicate DS_Init(s:DS_State, config:H_s.ConcreteConfiguration)
+  reads *
+{
+  && s.config == config
+  && H_s.ConcreteConfigToServers(s.config) == mapdomain(s.servers)
+  && H_s.ConcreteConfigInit(s.config)
+  && LEnvironment_Init(s.environment)
+  && (forall id :: id in s.servers ==> H_s.HostInit(s.servers[id], config, id))
+}
+  
+predicate DS_NextOneServer(s:DS_State, s':DS_State, id:EndPoint, ios:seq<LIoOp<EndPoint,seq<byte>>>)
+  requires id in s.servers
+  // reads *
+{
+  && id in s'.servers
+  && H_s.HostNext(s.servers[id], s'.servers[id], ios)
+  && s'.servers == s.servers[id := s'.servers[id]]
+}
+
+predicate DS_Next(s:DS_State, s':DS_State)
+  // reads *
+{
+  && s'.config == s.config
+  && LEnvironment_Next(s.environment, s'.environment)
+  && ValidPhysicalEnvironmentStep(s.environment.nextStep)
+  && if s.environment.nextStep.LEnvStepHostIos? && s.environment.nextStep.actor in s.servers then
+      DS_NextOneServer(s, s', s.environment.nextStep.actor, s.environment.nextStep.ios)
+    else
+      s'.servers == s.servers
+}
 }
