ironfleet/src/Dafny/Distributed/Impl/LiveSHT/Host.i.dfy
@@ -1,10 +1,14 @@
-include "../../Common/Framework/Host.s.dfy"
+// include "../../Common/Framework/Host.s.dfy"
 include "SchedulerImpl.i.dfy"
 include "CmdLineParser.i.dfy"
 
-module Host_i refines Host_s {
+module Host_i {
+// refines Host_s {
     import opened Collections__Sets_i
-
+import opened Native__Io_s
+import opened Environment_s 
+import opened Native__NativeTypes_s
+    
     import opened Common__NodeIdentity_i
     import opened Impl_Parameters_i
     import opened SHT__ConstantsState_i
@@ -24,6 +28,7 @@ module Host_i refines Host_s {
         provides HostInitImpl, HostNextImpl
     export All reveals *
 
+    predicate ArbitraryObject(o:object) { true }
 
     datatype CScheduler = CScheduler(ghost sched:LScheduler, scheduler_impl:SchedulerImpl?)
 
@@ -31,6 +36,7 @@ module Host_i refines Host_s {
     type ConcreteConfiguration = ConstantsState
 
     predicate HostStateInvariants(host_state:HostState, env:HostEnvironment)
+        reads *
     {
         host_state.scheduler_impl != null 
      && host_state.scheduler_impl.Valid() 
@@ -39,6 +45,7 @@ module Host_i refines Host_s {
     }
 
     predicate HostInit(host_state:HostState, config:ConcreteConfiguration, id:EndPoint)
+        reads *
     {
         host_state.scheduler_impl != null && host_state.scheduler_impl.Valid()
      && host_state.scheduler_impl.host.constants == config
@@ -83,6 +90,21 @@ module Host_i refines Host_s {
       ok:bool,
       host_state:HostState
       )
+  requires env.Valid()
+  requires env.ok.ok()
+  requires netc.IsOpen()
+  requires netc.env == env
+  requires ValidPhysicalAddress(EndPoint(netc.MyPublicKey()))
+  modifies set x:object | ArbitraryObject(x)     // Everything!
+  ensures  ok ==> env.Valid() && env.ok.ok()
+  ensures  ok ==> HostStateInvariants(host_state, env)
+  ensures  ok ==> var id := EndPoint(netc.MyPublicKey());
+                 var config := ParseCommandLineConfiguration(args);
+                 && id in ConcreteConfigToServers(config)
+                 && ConcreteConfigInit(config)
+                 && HostInit(host_state, config, id)
+  ensures  env.net.history() == old(env.net.history()) // Prohibit HostInitImpl from sending (and receiving) packets
+
     {
         var config:ConstantsState, my_index:uint64;
         var id := EndPoint(netc.MyPublicKey());
@@ -199,6 +221,22 @@ module Host_i refines Host_s {
         returns (ok:bool, host_state':HostState, 
                  ghost recvs:seq<NetEvent>, ghost clocks:seq<NetEvent>, ghost sends:seq<NetEvent>, 
                  ghost ios:seq<LIoOp<EndPoint, seq<byte>>>)
+  requires env.Valid() && env.ok.ok()
+  requires HostStateInvariants(host_state, env)
+  modifies set x:object | ArbitraryObject(x)     // Everything!
+  ensures  ok <==> env.Valid() && env.ok.ok()
+  ensures  ok ==> HostStateInvariants(host_state', env)
+  ensures  ok ==> HostNext(host_state, host_state', ios)
+  // Connect the low-level IO events to the spec-level IO events
+  ensures  ok ==> recvs + clocks + sends == ios
+  // These obligations enable us to apply reduction
+  // Even when !ok, if sent is non-empty, we need to return valid set of sent packets too
+  ensures  (ok || |sends| > 0) ==> env.net.history() == old(env.net.history()) + (recvs + clocks + sends)
+  ensures  forall e :: && (e in recvs ==> e.LIoOpReceive?) 
+                 && (e in clocks ==> e.LIoOpReadClock? || e.LIoOpTimeoutReceive?) 
+                 && (e in sends ==> e.LIoOpSend?)
+  ensures  |clocks| <= 1
+
     {
         var okay, netEventLog, abstract_ios := host_state.scheduler_impl.Host_Next_main();
         if okay {
