ironfleet/src/Dafny/Distributed/Services/SHT/Main.i.dfy
@@ -1,4 +1,4 @@
-include "../../Common/Framework/Main.s.dfy"
+// include "../../Common/Framework/Main.s.dfy"
 include "SHTDistributedSystem.i.dfy"
 include "../../Impl/LiveSHT/Host.i.dfy"
 include "../../Common/Collections/Maps2.s.dfy"
@@ -7,8 +7,9 @@ include "../../Protocol/Common/NodeIdentity.i.dfy"
 include "../../Protocol/LiveSHT/RefinementProof/SHTLemmas.i.dfy"
 include "Marshall.i.dfy"
 include "../../Protocol/SHT/Network.i.dfy"
+// module Main_i refines Main_s {
 
-module Main_i refines Main_s {
+module Main_i {
     import opened AS_s = AbstractServiceSHT_s`Spec
     import opened DS_s = SHT_DistributedSystem_i
     import opened DS_s.H_s
@@ -45,13 +46,16 @@ module Main_i refines Main_s {
     import opened Common__GenericMarshalling_i
     import opened Common__NetClient_i
     import opened Common__NodeIdentity_i
-    
+    import opened Native__Io_s
+    import opened Native__NativeTypes_s
+import opened Collections__Seqs_s
+
     export
         provides DS_s, Native__Io_s, Native__NativeTypes_s
         provides IronfleetMain
 
     predicate IsValidBehavior(config:ConcreteConfiguration, db:seq<DS_State>)
-        // reads *;
+        reads *;
     {
            |db| > 0
         && DS_Init(db[0], config)
@@ -1570,10 +1574,58 @@ module Main_i refines Main_s {
     }
 
     lemma RefinementProof(config:DS_s.H_s.ConcreteConfiguration, db:seq<DS_State>) returns (sb:seq<ServiceState>)
+        requires |db| > 0
+        requires DS_Init(db[0], config)
+        requires forall i {:trigger DS_Next(db[i], db[i+1])} :: 0 <= i < |db| - 1 ==> DS_Next(db[i], db[i+1])
+        ensures  |db| == |sb|
+        ensures  Service_Init(sb[0], Collections__Maps2_s.mapdomain(db[0].servers))
+        ensures  forall i {:trigger Service_Next(sb[i], sb[i+1])} :: 0 <= i < |sb| - 1 ==> sb[i] == sb[i+1] || Service_Next(sb[i], sb[i+1])
+        ensures  forall i :: 0 <= i < |db| ==> Service_Correspondence(db[i].environment.sentPackets, sb[i])
     {
         var db' := lemma_FixFinalEnvStep(config, db);
         sb := RefinementProofForFixedBehavior(config, db');
     }
 
-    
+
+method IronfleetMain(ghost env:HostEnvironment, netc:NetClient, args:seq<seq<byte>>)
+  requires env.Valid() && env.ok.ok()
+  requires env.net.history() == []
+  requires netc.IsOpen()
+  requires netc.env == env
+  requires ValidPhysicalAddress(EndPoint(netc.MyPublicKey()))
+  modifies set x:object | DS_s.H_s.ArbitraryObject(x)     // Everything!
+  decreases *
+{
+  var ok, host_state := DS_s.H_s.HostInitImpl(env, netc, args);
+  var config := DS_s.H_s.ParseCommandLineConfiguration(args);
+  var id := EndPoint(netc.MyPublicKey());
+  assert ok ==> DS_s.H_s.HostInit(host_state, config, id);
+
+  while (ok) 
+    invariant ok ==> DS_s.H_s.HostStateInvariants(host_state, env)
+    invariant ok ==> env.Valid() && env.ok.ok()
+    decreases *
+  {
+    ghost var old_net_history := env.net.history();
+    ghost var old_state := host_state;
+
+    ghost var recvs, clocks, sends, ios;
+    ok, host_state, recvs, clocks, sends, ios := DS_s.H_s.HostNextImpl(env, host_state);
+
+    if ok {
+      // Correctly executed one action
+      assert DS_s.H_s.HostNext(old_state, host_state, ios);
+
+      // Connect the low-level IO events to the spec-level IO events
+      assert recvs + clocks + sends == ios;
+
+      // These obligations enable us to apply reduction
+      assert env.net.history() == old_net_history + recvs + clocks + sends;
+      assert forall e :: && (e in recvs ==> e.LIoOpReceive?) 
+                   && (e in clocks ==> e.LIoOpReadClock? || e.LIoOpTimeoutReceive?) 
+                   && (e in sends ==> e.LIoOpSend?);
+      assert |clocks| <= 1;
+    }
+  }
+}
 }
